@prefix rdfs: <http://www.w3.org/2000/01/rdf-schema#> .
@prefix xsd: <http://www.w3.org/2001/XMLSchema#> .
@prefix owl: <http://www.w3.org/2002/07/owl#> .
@prefix tcs: <http://terminusdb.com/schema/tcs#> .
@prefix xdd: <http://terminusdb.com/schema/xdd#> .
@prefix terminus: <http://terminusdb.com/schema/terminus#> .

<http://terminusdb.com/schema/terminus>
  a owl:Ontology ;
  rdfs:label "Terminus DB Management Schema"@en ;
  rdfs:comment "Schema describing all of the structure of the documents (capabilities, roles, resources, users, databases) in the capability database used by Terminus DB to manage the internal state of the server and the databases it manages"@en ;
  tcs:rights "Copyright Data Chemist Ltd. 2017-2019"@en ;
  tcs:author "Gavin Mendel-Gleason"@en, "Kevin C. Feeney"@en;
  tcs:license <https://creativecommons.org/licenses/by-sa/2.0/>, <https://www.gnu.org/licenses/gpl-3.0.en.html> .

terminus:Agent
  rdfs:label "Agent"@en ;
  rdfs:comment "An agent is an abstraction of a thing that can have a capability"@en ;
  a owl:Class ;
  tcs:tag tcs:abstract ;
  rdfs:subClassOf tcs:Entity .

tcs:rights
  a owl:DatatypeProperty ;
  rdfs:range xsd:string ;
  rdfs:domain owl:Ontology ;
  rdfs:label "Rights"@en ;
  rdfs:comment "The statement of rights of the owner"@en .

tcs:author
  a owl:DatatypeProperty ;
  rdfs:domain owl:Ontology ;
  rdfs:range xsd:string ;
  rdfs:label "Author"@en ;
  rdfs:comment "The authors who developed the ontology"@en .

tcs:license
  a owl:ObjectProperty ;
  rdfs:domain owl:Ontology ;
  rdfs:range owl:Thing ;
  rdfs:label "License"@en ;
  rdfs:comment "The license governing the use of the resource"@en .

terminus:authority
  rdfs:label "Has Capability"@en ;
  rdfs:comment "A property that links an agent to a capability that they possess"@en ;
  a owl:ObjectProperty ;
  rdfs:domain terminus:Agent ;
  rdfs:range terminus:Capability .

terminus:Role
  rdfs:label "Role"@en ;
  rdfs:comment "A role is a collection of capabilities that can be allocated to any user"@en ;
  a owl:Class ;
  rdfs:subClassOf terminus:Agent .

terminus:User
  rdfs:label "User"@en ;
  rdfs:comment "A user of the database"@en ;
  a owl:Class ;
  rdfs:subClassOf terminus:Agent .

terminus:email
  rdfs:label "Email Address"@en ;
  rdfs:comment "A email address that allows the user to be contacted outside the system"@en ;
  a owl:DatatypeProperty ;
  rdfs:domain terminus:User ;
  rdfs:range xdd:email .

terminus:Capability
  rdfs:label "Capability"@en ;
  rdfs:comment "A capability confers access to a database or server action"@en ;
  tcs:tag tcs:abstract ;
  a owl:Class ;
  rdfs:subClassOf tcs:Entity.

terminus:ServerCapability
  rdfs:label "Server Capability"@en ;
  rdfs:comment "A capability to carry out some action on the server"@en ;
  a owl:Class ;
  rdfs:subClassOf terminus:RestrictServerCapability, terminus:Capability .

terminus:DatabaseCapability
  rdfs:label "Database Capability"@en ;
  rdfs:comment "A capability to carry out some action on a specific database"@en ;
  a owl:Class ;
  rdfs:subClassOf terminus:RestrictDBCapability, terminus:Capability.

terminus:authority_scope
  rdfs:label "Capability Scope"@en ;
  rdfs:comment "The scope of the capability - the resource that the capability applies to"@en ;
  a owl:ObjectProperty ;
  rdfs:domain terminus:Capability ;
  rdfs:range terminus:Resource .

terminus:resource_includes
  rdfs:label "Resource Inclusion"@en ;
  rdfs:comment "Resource A includes Resource B if A resource_includes B i.e. A Server might include a Database within its scope"@en ;
  a owl:ObjectProperty ;
  rdfs:domain terminus:Resource ;
  rdfs:range terminus:Resource .

terminus:RestrictServerCapability
  a owl:Restriction ;
  rdfs:label "Server Capabilities Apply to Servers"@en;
  rdfs:comment "Restricts the authority scope of the Server Capability to a Server Resource"@en;
  owl:onProperty terminus:authority_scope ;
  owl:allValuesFrom terminus:Server .

terminus:RestrictDBCapability
  a owl:Restriction ;
  rdfs:label "Database Capabilities Apply to DBs"@en;
  rdfs:comment "Restricts the authority scope of the Database Capability to a DB Resource"@en;
  owl:onProperty terminus:authority_scope ;
  owl:allValuesFrom terminus:Database .

terminus:action
  rdfs:label "Action"@en ;
  rdfs:comment "Refers to a specific API access call"@en ;
  a owl:ObjectProperty ;
  rdfs:domain terminus:Capability ;
  rdfs:range terminus:DBAction.

terminus:DBAction
  rdfs:label "DB Action"@en ;
  a owl:Class ;
  owl:oneOf (
   terminus:delete_database
   terminus:update_schema
   terminus:get_schema
   terminus:create_document
   terminus:get_document
   terminus:update_document
   terminus:delete_document
   terminus:class_frame
   terminus:woql_select
   terminus:woql_update
 ) .

terminus:delete_database
  rdfs:label "Delete Database"@en ;
  rdfs:comment "An action that deletes an entire database"@en ;
  a terminus:DBAction.

terminus:update_schema
  rdfs:label "Update Schema"@en ;
  rdfs:comment "An action that updates the DB schema"@en ;
  a terminus:DBAction.

terminus:get_schema
  rdfs:label "Get Schema"@en ;
  rdfs:comment "An action that fetches the DB Schema"@en ;
  a terminus:DBAction.

terminus:create_document
  rdfs:label "Create Document"@en ;
  rdfs:comment "An action that creates a new document"@en ;
  a terminus:DBAction.

terminus:get_document
  rdfs:label "Get Document"@en ;
  rdfs:comment "An action that retrieves a document from the DB"@en ;
  a terminus:DBAction.

terminus:update_document
  rdfs:label "Update Document"@en ;
  rdfs:comment "An action that updates the contents of a docoument"@en ;
  a terminus:DBAction.

terminus:delete_document
  rdfs:label "Delete Document"@en ;
  rdfs:comment "An action that deletes a document from the DB"@en ;
  a terminus:DBAction.

terminus:class_frame
  rdfs:label "Class Frame"@en ;
  rdfs:comment "An action that fetches a Frame JSON for the appropriate Class"@en ;
  a terminus:DBAction.

terminus:create_database
  rdfs:label "Create Database"@en ;
  rdfs:comment "An action which creates a new database"@en ;
  a terminus:DBAction.

terminus:woql_select
  rdfs:label "WOQL Select"@en ;
  rdfs:comment "An action which returns the results of a read-only query to the DB"@en ;
  a terminus:DBAction .

terminus:woql_update
  rdfs:label "WOQL Update"@en ;
  rdfs:comment "An action which returns the results of a read-write query to the DB"@en ;
  a terminus:DBAction .

terminus:Resource
  rdfs:label "Resource"@en ;
  rdfs:comment "A resource is a thing that can be accessed and given instructions and for which capabilities can be allocated"@en ;
  a owl:Class ;
  tcs:tag tcs:abstract ;
  rdfs:subClassOf tcs:Entity .

terminus:Database
  rdfs:label "Database"@en ;
  rdfs:comment "A resource representing a database hosted on the server"@en ;
  a owl:Class ;
  rdfs:subClassOf terminus:Resource .

terminus:allow_origin
  rdfs:label "Allow Requests from"@en ;
  rdfs:comment "Specify which domains can access this database from the web. Set to \"*\" for universal access. Sets the HTTP Access-Control-Allow-Origin header. "@en ;
  a owl:DatatypeProperty;
  rdfs:domain terminus:Resource;
  rdfs:range xsd:string.

terminus:Server
  rdfs:label "Server"@en ;
  rdfs:comment "A Resource Object Representing the Database Server itself"@en ;
  a owl:Class ;
  rdfs:subClassOf terminus:Resource .

terminus:schema
  a owl:DatatypeProperty ;
  rdfs:label "schema"@en ;
  rdfs:comment "A schema graph associated with the given database. All schema graphs are unioned."@en ;    
  rdfs:domain terminus:Database ;
  rdfs:range xsd:string .

terminus:instance
  a owl:DatatypeProperty ;
  rdfs:label "document"@en ;
  rdfs:comment "A document / instance graph associated with the given database. All instance graphs are unioned"@en ;
  rdfs:domain terminus:Database ;
  rdfs:range xsd:string .

terminus:inference
  a owl:DatatypeProperty ;
  rdfs:label "inference"@en ;
  rdfs:comment "An inference graph associated with the given database. All inference graphs are unioned"@en ;
  rdfs:domain terminus:Database ;
  rdfs:range xsd:string .

terminus:APIUpdate
  a owl:Class;
  rdfs:label "API Update"@en;
  rdfs:comment "A document that amounts to an update request, sent to the API"@en.

terminus:id
  a owl:DatatypeProperty ;
  rdfs:label "id"@en ;
  rdfs:comment "The universal identifier of the underlying asset of a given resource."@en ;
  rdfs:domain terminus:Resource ;
  rdfs:range xsd:anyURI .

terminus:document
  a owl:ObjectProperty;
  rdfs:label "Document"@en;
  rdfs:comment "The document being updated"@en;
  rdfs:domain terminus:APIUpdate;
  rdfs:range tcs:Entity.
  
terminus:user_key_hash
  a owl:DatatypeProperty;
  rdfs:label "User Key"@en;
  rdfs:comment "A user key for API authentication"@en;
  rdfs:domain terminus:User;
  rdfs:range xsd:string.

terminus:encoding
  rdfs:label "Encoding"@en ;
  rdfs:comment "The encoding that is used for a terminus document"@en ;
  a owl:ObjectProperty ;
  rdfs:domain terminus:APIUpdate ;
  rdfs:range terminus:DocumentEncoding.

terminus:DocumentEncoding
  rdfs:label "Document Endcoding"@en ;
  a owl:Class ;
  owl:oneOf (
   terminus:frame
   terminus:jsonld
   terminus:owl
 ) .  

terminus:frame
  rdfs:label "Frame"@en ;
  rdfs:comment "A document encoded as a JSON frame (complete with all available meta-data about its type)"@en ;
  a terminus:DocumentEncoding.

terminus:jsonld
  rdfs:label "JSON LD"@en ;
  rdfs:comment "Basic JSON-LD document encoding"@en ;
  a terminus:DocumentEncoding.

terminus:owl
  rdfs:label "OWL"@en ;
  rdfs:comment "Schema encoding - Web Ontology Langauge"@en ;
  a terminus:DocumentEncoding.
